Trying to show -1*-1 = 1. WIP.

Coq/OddAndEvenParts/OddAndEvenPartsGeneral.v
@@ -31,7 +31,7 @@ Section FiniteFieldModulo3.
     end.
 
   (* Define the negation operation modulo 3 *)
-  Definition F3opp (x : F3) : F3 :=
+  Definition F3add_inv (x : F3) : F3 :=
     match x with
     | F0 => F0
     | F1 => F2
@@ -46,7 +46,7 @@ Section FiniteFieldModulo3.
     | F2 => F2
     end.
 
-  Definition F3sub (x y : F3) : F3 := F3add x (F3opp y).
+  Definition F3sub (x y : F3) : F3 := F3add x (F3add_inv y).
 
   Definition F3div (x y : F3) : F3 := F3mul x (F3inv y).
 
@@ -54,7 +54,7 @@ Section FiniteFieldModulo3.
   Variable F : Type.
   Variable zero one : F.
   Variable add mul sub : F -> F -> F.
-  Variable opp inv : F -> F.
+  Variable add_inv inv : F -> F.
   Variable div : F -> F -> F.
 
   Declare Scope field_scope.
@@ -64,23 +64,23 @@ Section FiniteFieldModulo3.
   Notation "2" := (add one one) : field_scope.
   Notation "x * y" := (mul x y) : field_scope.
   Notation "x - y" := (sub x y) : field_scope.
-  Notation "- x" := (opp x) : field_scope.
+  Notation "- x" := (add_inv x) : field_scope.
   Notation "/ x" := (inv x) : field_scope.
 
   Open Scope field_scope.
   
   Variable add_assoc : forall x y z : F, (x + y) + z = x + (y + z).
   Variable add_0_r : forall x : F, x + 0 = x.
-  Variable add_opp_r : forall x : F, x + (- x) = 0.
+  Variable add_inv_r : forall x : F, x + (- x) = 0.
   Variable add_comm : forall x y : F, x + y = y + x.
   Variable mul_1_l : forall x : F, 1 * x = x.
   Variable mul_1_r : forall x : F, x * 1 = x.
-  Variable inv_mul : forall x : F, x <> 0 -> x * (/ x) = 1.
+  Variable mul_inv : forall x : F, x <> 0 -> x * (/ x) = 1.
   Variable mul_add_distr_l : forall x y z : F, x * (y + z) = (x * y) + (x * z).
   Variable mul_add_distr_r : forall x y z : F, (x + y) * z = x * z + y * z.
   Variable sub_def : forall x y : F, x - y = x + (- y).
   Variable mul_sub_distr_r : forall r1 r2 r3 : F, (r2 - r3)*r1 = r2 * r1 - r3 * r1.
-  Variable opp_sub_distr : forall r1 r2 : F, - (r1 - r2) = r2 - r1.
+  Variable add_inv_sub_distr : forall r1 r2 : F, - (r1 - r2) = r2 - r1.
 
   Variable neq_2_0 : 2 <> 0.
 
@@ -92,18 +92,45 @@ Section FiniteFieldModulo3.
     reflexivity.
   Qed.
 
-  Lemma opp_involutive : forall x : F, - (- x) = x.
+  Lemma add_inv_involutive : forall x : F, - (- x) = x.
   Proof.
     intro.
     rewrite <- add_0_r with (x := --x).
-    rewrite <- add_opp_r with (x := x).
+    rewrite <- add_inv_r with (x := x).
     rewrite add_comm with (x := x) (y := -x).
     rewrite <- add_assoc with (x := --x) (y := -x) (z := x).
     rewrite add_comm with (x := --x) (y := -x).
-    rewrite add_opp_r with (x := -x).
+    rewrite add_inv_r with (x := -x).
     rewrite add_0_l.
     reflexivity.
   Qed.
+
+  Definition mul_comm := forall x y : F, x * y = y * x.
+  Definition mul_assoc := forall x y z : F, (x * y) * z = x * (y * z).
+  Definition mul_inv_nonzero := forall x : F, x <> 0 -> /x <> 0.
+
+  Lemma mul_inv_involutive (Hmul_comm : mul_comm) (Hmul_assoc : mul_assoc) (Hmul_inv_nonzero : mul_inv_nonzero) : forall x : F, x <> 0 -> //x = x.
+  Proof.
+    intros.
+    rewrite <- mul_1_r with (x := //x).
+    rewrite <- mul_inv with (x := x).
+    rewrite Hmul_comm with (x := x) (y := /x).
+    rewrite <- Hmul_assoc with (x := //x) (y := /x) (z := x).
+    rewrite Hmul_comm with (x := //x) (y := /x).
+    rewrite mul_inv with (x := /x).
+    rewrite mul_1_l.
+    reflexivity.
+    - apply Hmul_inv_nonzero.
+      apply H.
+    - apply H.
+  Qed.
+
+  Lemma neg_1_sqr : (- (1)) * (- (1)) = (1).
+  Proof.
+    rewrite <- mul_inv with (x := -(1)) at 3.
+    - f_equal.
+      rewrite <- mul_1_l.
+ Admitted.
 
   (* Definitions of even and odd parts for functions over a field *)
   Definition evenPart (f : F -> F) : F -> F := fun x => (f x + f (- x)) * / 2.
@@ -118,7 +145,7 @@ Section FiniteFieldModulo3.
     intros.
     unfold isEven, evenPart.
     intros.
-    rewrite opp_involutive.
+    rewrite add_inv_involutive.
     rewrite (add_comm (f x) (f (- x))).
     reflexivity.
   Qed.
@@ -128,9 +155,9 @@ Section FiniteFieldModulo3.
     intros.
     unfold isOdd, oddPart.
     intros.
-    rewrite opp_involutive.
+    rewrite add_inv_involutive.
     rewrite mul_sub_distr_r with (r1 := /2) (r2 := f x) (r3 := f (-x)).
-    rewrite opp_sub_distr with (r1 := f x * /2) (r2 := f (-x) * /2).
+    rewrite add_inv_sub_distr with (r1 := f x * /2) (r2 := f (-x) * /2).
     rewrite <- mul_sub_distr_r with (r1 := /2) (r2 := f (-x)) (r3 := f x).
     reflexivity.
   Qed.
@@ -164,7 +191,7 @@ Section FiniteFieldModulo3.
     rewrite add_comm with (x := f (- x) * /2) (y := f x * /2).
     rewrite add_assoc.
     rewrite add_assoc.
-    rewrite add_opp_r.
+    rewrite add_inv_r.
     rewrite add_0_r.
     (*
       f x = f x * / 2 + f x * / 2
@@ -173,7 +200,7 @@ Section FiniteFieldModulo3.
     rewrite <- mul_add_distr_l with (x := f x) (y := /2) (z := /2).
     rewrite <- mul_1_l with (x := /2).
     rewrite <- mul_add_distr_r.
-    rewrite inv_mul by apply neq_2_0.
+    rewrite mul_inv by apply neq_2_0.
     rewrite mul_1_r.
     (*
       f x = f x
@@ -194,7 +221,7 @@ Module ApplyFiniteFieldModulo3.
   Definition add := F3add.
   Definition mul := F3mul.
   Definition sub := F3sub.
-  Definition opp := F3opp.
+  Definition add_inv := F3add_inv.
   Definition inv := F3inv.
   Definition div := F3div.
 
@@ -210,7 +237,7 @@ Module ApplyFiniteFieldModulo3.
   Notation "2" := (add one one) : field_scope.
   Notation "x * y" := (mul x y) : field_scope.
   Notation "x - y" := (sub x y) : field_scope.
-  Notation "- x" := (opp x) : field_scope.
+  Notation "- x" := (add_inv x) : field_scope.
   Notation "/ x" := (inv x) : field_scope.
 
   Open Scope field_scope.
@@ -230,9 +257,9 @@ Module ApplyFiniteFieldModulo3.
     intros. unfold add, zero, F3add. destruct x; reflexivity.
   Qed.
 
-  Definition add_opp_r : forall x : F, x + (- x) = 0.
+  Definition add_inv_r : forall x : F, x + (- x) = 0.
   Proof.
-    intros. unfold add, opp, zero, F3add, F3opp. destruct x; reflexivity.
+    intros. unfold add, add_inv, zero, F3add, F3add_inv. destruct x; reflexivity.
   Qed.
 
   Definition mul_1_l : forall x : F, (1 * x) = x.
@@ -257,55 +284,61 @@ Module ApplyFiniteFieldModulo3.
 
   Definition sub_def : forall x y : F, (x - y) = (x + (- y)).
   Proof.
-    intros. unfold sub, add, opp, F3sub, F3add, F3opp. reflexivity.
+    intros. unfold sub, add, add_inv, F3sub, F3add, F3add_inv. reflexivity.
   Qed.
 
-  Definition opp_involutive : forall x : F, - (- x) = x.
+  Definition add_inv_involutive : forall x : F, - (- x) = x.
   Proof.
-    intros. unfold opp, F3opp. destruct x; reflexivity.
+    intros. unfold add_inv, F3add_inv. destruct x; reflexivity.
   Qed.
 
-  Definition inv_mul : forall x : F, ~ x = zero -> (x * (/ x)) = one.
+  Definition mul_inv : forall x : F, ~ x = zero -> (x * (/ x)) = one.
   Proof.
     intros. unfold mul, inv, one, F3mul, F3inv. destruct x; try contradiction; reflexivity.
   Qed.
 
   Definition mul_sub_distr_r : forall r1 r2 r3 : F, (r2 - r3) * r1 = (r2 * r1) - (r3 * r1).
   Proof.
-    intros. unfold mul, sub, F3mul, F3sub, F3add, F3opp. destruct r1, r2, r3; reflexivity.
+    intros. unfold mul, sub, F3mul, F3sub, F3add, F3add_inv. destruct r1, r2, r3; reflexivity.
   Qed.
 
-  Definition opp_sub_distr : forall r1 r2 : F, - (r1 - r2) = r2 - r1.
+  Definition add_inv_sub_distr : forall r1 r2 : F, - (r1 - r2) = r2 - r1.
   Proof.
-    intros. unfold sub, opp, F3sub, F3add, F3opp. destruct r1, r2; reflexivity.
+    intros. unfold sub, add_inv, F3sub, F3add, F3add_inv. destruct r1, r2; reflexivity.
   Qed.
 
   (* Define a polynomial function f(x) = x^2 + x *)
   Definition poly1 (x : F) : F := add (mul x x) x.
 
+  (* Example poly1EventPart (x : F) : evenPart F F1 add mul add_inv inv poly1 x = mul x x.
+  Proof.
+    unfold evenPart, poly1.
+    
+  Qed. *)
+
   (* Apply the theorems to the finite field modulo 3 *)
-  Compute (evenPart F F1 add mul opp inv poly1 F0).
+  Compute (evenPart F F1 add mul add_inv inv poly1 F0).
   (* F0 *)
 
-  Compute (oddPart F F1 add mul sub opp inv poly1 F0).
+  Compute (oddPart F F1 add mul sub add_inv inv poly1 F0).
   (* F0 *)
 
-  Compute (evenPart F F1 add mul opp inv poly1 F1).
+  Compute (evenPart F F1 add mul add_inv inv poly1 F1).
   (* F1 *)
 
-  Compute (oddPart F F1 add mul sub opp inv poly1 F1).
+  Compute (oddPart F F1 add mul sub add_inv inv poly1 F1).
   (* F1 *)
 
-  Compute (evenPart F F1 add mul opp inv poly1 F2).
+  Compute (evenPart F F1 add mul add_inv inv poly1 F2).
   (* F1 *)
 
-  Compute (oddPart F F1 add mul sub opp inv poly1 F2).
+  Compute (oddPart F F1 add mul sub add_inv inv poly1 F2).
   (* F2 *)
 
   (* Example to verify the sum of even and odd parts equals the original polynomial *)
-  Example poly_even_odd_sum : forall x : F, poly1 x = add (evenPart F F1 add mul opp inv poly1 x) (oddPart F F1 add mul sub opp inv poly1 x).
+  Example poly_even_odd_sum : forall x : F, poly1 x = add (evenPart F F1 add mul add_inv inv poly1 x) (oddPart F F1 add mul sub add_inv inv poly1 x).
   Proof.
-    apply (fIsEvenPlusOdd F F0 F1 add mul sub opp inv add_assoc add_0_r add_opp_r add_comm mul_1_l mul_1_r inv_mul mul_add_distr_l mul_add_distr_r sub_def mul_sub_distr_r neq_2_0 poly1).
+    apply (fIsEvenPlusOdd F F0 F1 add mul sub add_inv inv add_assoc add_0_r add_inv_r add_comm mul_1_l mul_1_r mul_inv mul_add_distr_l mul_add_distr_r sub_def mul_sub_distr_r neq_2_0 poly1).
   Qed.
 
 End ApplyFiniteFieldModulo3.
